common/Values.v
@@ -724,16 +724,6 @@ Definition xorl (v1 v2: val): val :=
   | _, _ => Vundef
   end.
 
-Definition val_shift_lng_mask (v : int) : int :=
-  Int.and v (Int.repr 63).
-
-(* TODO: Move to Int to make this general across Cop.v and here *)
-Theorem lng_mask_size_val_ident:
-forall v : int,
-(*Int.ltu v Int64.iwordsize' = true -> val_shift_lng_mask v = v.*)
-(Int.unsigned v) < Int64.zwordsize -> val_shift_lng_mask v = v.
-Proof. Admitted.
-
 Definition shll (v1 v2: val): val :=
   match v1, v2 with
   | Vlong n1, Vint n2 => Vlong(Int64.shl' n1 (val_shift_lng_mask n2))
